Auto/Lib/BoolExtra.lean
@@ -9,6 +9,12 @@ theorem Bool.ne_true_of_eq_false {a : Bool} : a = false → a ≠ true := by
 theorem Bool.eq_false_eq_not_eq_true {a : Bool} : (a ≠ true) = (a = false) := by
   cases a <;> decide
 
+theorem Bool.and_eq_false (a b : Bool) : ((a && b) = false) = ((a = false) ∨ (b = false)) := by
+  cases a <;> cases b <;> decide
+
+theorem Bool.or_eq_false (a b : Bool) : ((a || b) = false) = ((a = false) ∧ (b = false)) := by
+  cases a <;> cases b <;> decide
+
 theorem Bool.and_comm {a b : Bool} : (a && b) = (b && a) := by
   cases a <;> cases b <;> decide
 
